theories/examples/lazy.v
@@ -24,7 +24,7 @@ Definition eager α : expr :=
   (λ:"_u", "b").
 
 Section proofs.
-  Context `{!prelocGS Σ, !logrel_na_invs Σ}.
+  Context `{!prelogrelGS Σ}.
   Context `{!lockG Σ}.
 
   Definition coinN := nroot.@"coins".
@@ -34,7 +34,7 @@ Section proofs.
     e1 = #lbl:α -> e2 = #lbl:β ->
     α ↪ (b::bs) ∗ β ↪ₛ (b::bs')
     -∗ REL lazy e1 << eager e2 : lrel_unit → lrel_bool.
-  Proof using lockG0 prelocGS0 Σ.
+  Proof using lockG0 prelogrelGS0 Σ.
     iIntros (-> ->) "[Hα Hβ]". rewrite /lazy /eager.
     rel_alloc_l l as "Hl" ; rel_pures_l ; rel_flip_r.
     rel_apply_l (refines_newlock_l coinN
@@ -61,7 +61,7 @@ Section proofs.
 
   Lemma lazy_eager_refinement' :
     ⊢ REL lazy' << eager' : lrel_unit → lrel_bool.
-  Proof using lockG0 prelocGS0 Σ.
+  Proof using lockG0 prelogrelGS0 Σ.
     rewrite /lazy' /eager'.
     rel_alloctape_l α as "Hα".
     rel_alloctape_r β as "Hβ".
@@ -74,14 +74,14 @@ Section proofs.
   Lemma lazy_eager_refinement'' α β :
     (REL α << β : lrel_tape)
       ⊢ REL lazy α << eager β : lrel_unit → lrel_bool.
-  Proof using lockG0 prelocGS0 Σ.
+  Proof using lockG0 prelogrelGS0 Σ.
   Admitted.
 
   Lemma eager_lazy_refinement e1 e2 α β b bs bs' :
     e1 = #lbl:α -> e2 = #lbl:β ->
     α ↪ (b::bs) ∗ β ↪ₛ (b::bs')
     -∗ REL eager e1 << lazy e2 : lrel_unit → lrel_bool.
-  Proof using lockG0 prelocGS0 Σ.
+  Proof using lockG0 prelogrelGS0 Σ.
     iIntros (-> ->) "[Hα Hβ]". rewrite /lazy /eager.
     rel_alloc_r l as "Hl" ; rel_pures_r ; rel_flip_l.
     rel_apply_r (refines_newlock_r).
@@ -110,7 +110,7 @@ Section proofs.
 
   Lemma eager_lazy_refinement' :
     ⊢ REL eager' << lazy' : lrel_unit → lrel_bool.
-  Proof using lockG0 prelocGS0 Σ.
+  Proof using lockG0 prelogrelGS0 Σ.
     rewrite /lazy' /eager'.
     rel_alloctape_l α as "Hα" ; rel_alloctape_r β as "Hβ".
     rel_pures_l ; rel_pures_r.
